Try to study par_seq lemma at smaller scale.

theories/SLOT/Ensemble.v
@@ -2,7 +2,8 @@ From Coq Require Import
      List.
 
 From LibTx Require Import
-     Hoare.
+     Permutation
+     SLOT.Hoare.
 
 Import ListNotations.
 
@@ -67,6 +68,35 @@ Section props.
     apply hoare_concat with (mid0 := mid); auto.
   Qed.
 
+  Section perm_props.
+    Context (can_swap : TE -> TE -> Prop).
+
+    Definition perm t1 t2 := Permutation can_swap (t1 ++ t2).
+
+    (* Let's try and prove the simplest case... If it's true,
+    that'd be pretty epic, as it would allow using dynamic programming
+    techniques for exploration of schedulings *)
+    Goal forall P Q R te0 te1 te2,
+        -{{P}} perm [te0] [te1] {{Q}} ->
+        -{{Q}} perm [te0] [te2] {{R}} ->
+        -{{P}} perm [te0] [te1; te2] {{R}}.
+    Proof.
+      intros. intros t Ht.
+      inversion_ Ht.
+      Focus 2.
+      inversion_ H2. simpl in *.
+    Abort.
+
+    Lemma hoare_perm_seq : forall P Q R t0 t1 t2,
+        -{{P}} perm t0 t1 {{Q}} ->
+        -{{Q}} perm t0 t2 {{R}} ->
+        -{{P}} perm t0 (t1 ++ t2) {{R}}.
+    Abort. (* This is _likely_ wrong:
+            P t1:[a b] Q t2:[c d] R
+              t0: [A         B]
+            *)
+  End perm_props.
+
   Lemma e_hoare_par_seq : forall e1 e2 e P Q R,
       -{{P}} e1 |> e {{Q}} ->
       -{{Q}} e2 |> e {{R}} ->
@@ -74,5 +104,5 @@ Section props.
   Proof.
     intros *. intros H1 H2 t Ht s s' Hss' Hpre.
     destruct Ht as [t1 t2 t Ht1 Ht2 Hint].
-  Abort.
+  Abort. (* This is wrong? *)
 End props.
